Clean up a bit

ContractExamples/FStar/CallOption.fst
@@ -171,66 +171,57 @@ let findRoot #n iData #nAuditPathHashes {location=location;hashes=hashes} =
   do optRoot' <-- optRoot;
   ret @ O.maybe (E.failw "Can't hash input data") (E.ret) optRoot'
 
-val initializeTx : utxo -> hash -> outpoint -> cost (result transactionSkeleton) 55
+val initializeTx : utxo -> hash -> outpoint -> cost (result transactionSkeleton) 56
 let initializeTx utxo cHash outpoint =
-      (do numeraire <-- numeraire;
-      let open ET in
-      do (pt, oput) <-- tryAddPoint outpoint utxo;
-      if oput.spend.asset = numeraire
-      then      // Initialize with data output
-        let initialState : state =
-          {
-            tokensIssued=0UL;
-            collateral=oput.spend.amount;
-            counter=0UL;
-          } in
-        do initialStateData <-- retT @ encodeState initialState;
-        let dataOutputLock = ContractLock cHash 3 initialStateData in
-        let dataOutput = {lock=dataOutputLock;spend=oput.spend} in
-        ret @ Tx V[pt] V[dataOutput] None
-      else
-      autoFailw "Can't initialize with this asset.")
+    let open ET in
+    do numeraire <-- retT numeraire;
+    do (pt, oput) <-- tryAddPoint outpoint utxo;
+    if oput.spend.asset = numeraire
+    then      // Initialize with data output
+      let initialState : state =
+        {
+          tokensIssued=0UL;
+          collateral=oput.spend.amount;
+          counter=0UL;
+        } in
+      do initialStateData <-- retT @ encodeState initialState;
+      let dataOutputLock = ContractLock cHash 3 initialStateData in
+      let dataOutput = {lock=dataOutputLock;spend=oput.spend} in
+      ret @ Tx V[pt] V[dataOutput] None
+    else
+    autoFailw "Can't initialize with this asset."
 
 val collateralizeTx :
     utxo
     -> hash
     -> outpoint
     -> outpoint
-    -> cost (result transactionSkeleton) 129
+    -> cost (result transactionSkeleton) 130
 let collateralizeTx utxo cHash outpoint0 outpoint1 =
-      do numeraire <-- numeraire;
-      let open ET in
-      do (pt0, dataOutput)     <-- tryAddPoint outpoint0 utxo;
-      do (pt1, newFundsOutput) <-- tryAddPoint outpoint1 utxo;
-      if dataOutput.spend.asset = numeraire && newFundsOutput.spend.asset = numeraire
-      then
-        begin match dataOutput.lock, newFundsOutput.lock with
-        | ContractLock h1 3 currentStateData, ContractLock h2 _ _ ->
-            if h1 <> cHash || h2 <> cHash
-            then autoFailw "Locked to wrong contract"
-            else begin
-            do currentState <-- decodeState currentStateData;
-            do newCollateral <-- currentState.collateral +?^ newFundsOutput.spend.amount;
-            let newState = {
-              tokensIssued = currentState.tokensIssued;
-              collateral = newCollateral;
-              counter = currentState.counter +%^ 1UL;   // We actually prefer modular arithmetic for the counter
-            } in
-            do newStateData <-- retT @ encodeState newState;
-            let newDataOutputLock = ContractLock cHash 3 newStateData in
-            let newDataOutput =
-              {
-                lock=newDataOutputLock;
-                spend={asset=numeraire;amount=newCollateral}
-              } in
-            ret @ Tx
-                    V[pt0; pt1]
-                    V[newDataOutput]
-                    None
-            end
-        | _,_ -> autoFailw "Inputs not locked to this contract!"
+    let open ET in
+    do numeraire <-- retT numeraire;
+    do (pt0, dataOutput)     <-- tryAddPoint outpoint0 utxo;
+    do (pt1, newFundsOutput) <-- tryAddPoint outpoint1 utxo;
+    if dataOutput.spend.asset <> numeraire || newFundsOutput.spend.asset <> numeraire
+    then autoFailw "Can't use these asset types for Collateralize" else
+    match dataOutput.lock, newFundsOutput.lock with
+    | ContractLock h1 3 currentStateData, ContractLock h2 _ _ ->
+        if h1 <> cHash || h2 <> cHash
+        then autoFailw "Locked to wrong contract" else begin
+        do  currentState <-- decodeState currentStateData;
+        do newCollateral <-- currentState.collateral +?^ newFundsOutput.spend.amount;
+        let newState = { tokensIssued = currentState.tokensIssued;
+                         collateral = newCollateral;
+                         counter = currentState.counter +%^ 1UL } in  // We actually prefer modular arithmetic for the counter
+        do newStateData <-- retT @ encodeState newState;
+        let newDataOutputLock = ContractLock cHash 3 newStateData in
+        let newDataOutput = { lock=newDataOutputLock;
+                              spend={asset=numeraire;amount=newCollateral} } in
+        ret @ Tx V[pt0; pt1]
+                 V[newDataOutput]
+                 None
         end
-      else autoFailw "Can't use these asset types for Collateralize"
+    | _,_ -> autoFailw "Inputs not locked to this contract!"
 
 val buyTx :
     utxo
@@ -238,105 +229,78 @@ val buyTx :
     -> outpoint
     -> outpoint
     -> outputLock
-    -> cost (result transactionSkeleton) 146
+    -> cost (result transactionSkeleton) 147
 let buyTx utxo cHash outpoint0 outpoint1 lk =
-      do numeraire <-- numeraire;
-      let open ET in
-      do (pt0, dataOutput)     <-- tryAddPoint outpoint0 utxo;
-      do (pt1, purchaseOutput) <-- tryAddPoint outpoint0 utxo;
-      if dataOutput.spend.asset = numeraire && purchaseOutput.spend.asset = numeraire
-      then
-      begin match dataOutput.lock, purchaseOutput.lock with
-      | ContractLock h1 3 currentStateData, ContractLock h2 _ _ ->
-          if h1 <> cHash || h2 <> cHash
-          then autoFailw "Locked to wrong contract"
-          else begin
-          do currentState <-- decodeState currentStateData;
-          do newCollateral <--currentState.collateral +?^ purchaseOutput.spend.amount;
-          let newTokens = purchaseOutput.spend.amount /^ price in   //downwards rounding
-          do tokensIssued <-- currentState.tokensIssued +?^ newTokens;
-          let newState = {
-            tokensIssued = tokensIssued;
-            collateral = newCollateral;
-            counter = currentState.counter;
-          } in        //TODO: return to sender with insufficient collateral
-          do newStateData <-- retT @ encodeState newState;
-          let newDataOutputLock = ContractLock cHash 3 newStateData in
-          let newDataOutput =
-            {
-              lock=newDataOutputLock;
-              spend={asset=numeraire;amount=newCollateral}
-            } in
-          let buyersOutput =
-            {
-              lock=lk;
-              spend={asset=cHash;amount=newTokens}
-            } in
-          ret @ Tx
-                  V[pt0; pt1]
-                  V[newDataOutput; buyersOutput]
-                  None
-          end
-      | _,_ -> autoFailw "Incorrect data or purchase lock"
-      end
-      else autoFailw "Can't buy with these assets."
+    let open ET in
+    do numeraire <-- retT numeraire;
+    do (pt0, dataOutput)     <-- tryAddPoint outpoint0 utxo;
+    do (pt1, purchaseOutput) <-- tryAddPoint outpoint0 utxo;
+    if dataOutput.spend.asset <> numeraire || purchaseOutput.spend.asset <> numeraire
+    then autoFailw "Can't buy with these assets." else
+    match dataOutput.lock, purchaseOutput.lock with
+    | ContractLock h1 3 currentStateData, ContractLock h2 _ _ ->
+        if h1 <> cHash || h2 <> cHash
+        then autoFailw "Locked to wrong contract" else begin
+        do currentState <-- decodeState currentStateData;
+        do newCollateral <--currentState.collateral +?^ purchaseOutput.spend.amount;
+        let newTokens = purchaseOutput.spend.amount /^ price in   //downwards rounding
+        do tokensIssued <-- currentState.tokensIssued +?^ newTokens;
+        let newState = { tokensIssued = tokensIssued;
+                         collateral = newCollateral;
+                         counter = currentState.counter } in        //TODO: return to sender with insufficient collateral
+        do newStateData <-- retT @ encodeState newState;
+        let newDataOutputLock = ContractLock cHash 3 newStateData in
+        let newDataOutput = { lock=newDataOutputLock;
+                              spend={asset=numeraire;amount=newCollateral} } in
+        let buyersOutput = { lock=lk; spend={asset=cHash;amount=newTokens} } in
+        ret @ Tx V[pt0; pt1]
+                 V[newDataOutput; buyersOutput]
+                 None
+        end
+    | _,_ -> autoFailw "Incorrect data or purchase lock"
 
 val restOfEx :
           hash -> pointedOutput -> pointedOutput -> pointedOutput
           -> U64.t
           -> outputLock
-          -> cost (result transactionSkeleton) 124
-let restOfEx
-        cHash
-        (pt1,dataOutput) (pt2,tokenOutput) (pt3,oracleOutput)
-        spot
-        payoffOutputLock =
-        begin
-          do numeraire <-- numeraire;
-          let open ET in
-          let open U64 in
-          if dataOutput.spend.asset <> numeraire || tokenOutput.spend.asset <> cHash
-          then autoFailw "Can't exercise with these assets."
-          else
-          match dataOutput.lock, tokenOutput.lock with
-          | ContractLock h1 3 currentStateData, ContractLock h2 _ _ ->
-              if h1 <> cHash || h2 <> cHash
-              then autoFailw "Locked to wrong contract"
-              else if spot <=^ strike then autoFailw "Spot price lower than strike."
-              else
-              let payoff = spot -^ strike in
-              begin
-              do totalPayoff <-- O.maybe
-                                  (autoFailw "Overflow")
-                                  (ET.ret)
-                                  (tokenOutput.spend.amount *?^ payoff);
-                do currentState <-- decodeState currentStateData;
-                let newCollateral = currentState.collateral -%^ totalPayoff in
-                let newState = {
-                  tokensIssued = currentState.tokensIssued -%^ tokenOutput.spend.amount; //TODO: modular
-                  collateral = newCollateral;
-                  counter = currentState.counter;
-                } in
-                //TODO: return to sender with insufficient collateral
-                do newStateData <-- retT @ encodeState newState;
-                let newDataOutputLock = ContractLock cHash 3 newStateData in
-                let newDataOutput =
-                  {
-                    lock=newDataOutputLock;
-                    spend={asset=numeraire;amount=newCollateral}
-                  } in
-                let payoffOutput =
-                  {
-                    lock=payoffOutputLock;
-                    spend={asset=numeraire;amount=totalPayoff}
-                  } in
-                ret @ Tx
-                        V[pt1; pt2]
-                        V[newDataOutput; payoffOutput]
-                        None
-              end
-          | _, _ -> autoFailw "Incorrect data or exercise(token) lock"
-         end
+          -> cost (result transactionSkeleton) 125
+let restOfEx cHash
+             (pt1,dataOutput) (pt2,tokenOutput) (pt3,oracleOutput)
+             spot
+             payoffOutputLock =
+    let open ET in
+    let open U64 in
+    do numeraire <-- retT numeraire;
+    if dataOutput.spend.asset <> numeraire || tokenOutput.spend.asset <> cHash
+    then autoFailw "Can't exercise with these assets." else
+    match dataOutput.lock, tokenOutput.lock with
+    | ContractLock h1 3 currentStateData, ContractLock h2 _ _ ->
+        if h1 <> cHash || h2 <> cHash
+        then autoFailw "Locked to wrong contract" else
+        if spot <=^ strike
+        then autoFailw "Spot price lower than strike." else begin
+        let payoff = spot -^ strike in
+        do totalPayoff <-- O.maybe
+                            (autoFailw "Overflow")
+                            (ET.ret)
+                            (tokenOutput.spend.amount *?^ payoff);
+        do currentState <-- decodeState currentStateData;
+        let newCollateral = currentState.collateral -%^ totalPayoff in
+        let newState = { tokensIssued = currentState.tokensIssued -%^ tokenOutput.spend.amount; //TODO: modular
+                         collateral = newCollateral;
+                         counter = currentState.counter } in
+        //TODO: return to sender with insufficient collateral
+        do newStateData <-- retT @ encodeState newState;
+        let newDataOutputLock = ContractLock cHash 3 newStateData in
+        let newDataOutput = { lock=newDataOutputLock;
+                              spend={asset=numeraire;amount=newCollateral} } in
+        let  payoffOutput = { lock=payoffOutputLock;
+                              spend={asset=numeraire;amount=totalPayoff} } in
+        ret @ Tx V[pt1; pt2]
+                 V[newDataOutput; payoffOutput]
+                 None
+        end
+    | _, _ -> autoFailw "Incorrect data or exercise(token) lock"
 
 val exerciseTx :
           utxo -> hash
@@ -347,89 +311,65 @@ val exerciseTx :
           -> (path:auditPath nAuditPathHashes)
           -> outputLock
           -> cost (result transactionSkeleton)
-                   M.((nUnderlyingAssetBytes+3) * 384 + 1291 + nAuditPathHashes)
+                   M.((nUnderlyingAssetBytes+3) * 384 + 1292 + nAuditPathHashes)
 
 let exerciseTx
           utxo
           cHash
           outpoint0 outpoint1 outpoint2
           #nUnderlyingAssetBytes
-          {
-                underlying=underlyingBytes;
-                price=price;
-                timestamp=timestamp;
-                nonce=nonce
-          }
+          { underlying=underlyingBytes;
+            price=price;
+            timestamp=timestamp;
+            nonce=nonce }
           #nAuditPathHashes
           auditPath
           payoffOutputLock =
-          begin
-          let open ET in
-          do (pt0, dataOutput)   <-- tryAddPoint outpoint0 utxo;
-          do (pt1, tokenOutput)  <-- tryAddPoint outpoint1 utxo;
-          do (pt2, oracleOutput) <-- tryAddPoint outpoint2 utxo;
-          let dataToHash  =
-            (Data4 nUnderlyingAssetBytes 1 1 1
-              (ByteArray nUnderlyingAssetBytes underlyingBytes)
-              (UInt64 price)
-              (UInt64 timestamp)
-              (Hash nonce)) in
-          // Validate data about the underlying against the Oracle's commitment
-          do expectedRoot <-- (
-            findRoot
-                                dataToHash
-                                auditPath
-                              ) ;
-          match oracleOutput with
-          | {
-              lock=(ContractLock oHash 1 (Hash mroot));
-              spend={asset=oHash2}
-            } ->
-            do oracleHash <-- retT @ oracleHash;
-            if oHash <> oracleHash then autoFailw "Incorrect oracle ID"
-            else if oHash2 <> oracleHash then autoFailw "Wrong oracle asset type"
-            else
-            if not (expectedRoot = mroot) then
-              autoFailw "wrong root"
-            else if nUnderlyingAssetBytes <> 32 then autoFailw "Limitation: symbol must be 32 bytes."
-            else begin
-            do underlyingSymbol <-- retT @ underlyingSymbol;
-            if underlyingBytes <> underlyingSymbol then
-              autoFailw "Trying to use the wrong underlying!"
-            else
-              restOfEx
-                cHash
-                (pt0,dataOutput) (pt1,tokenOutput) (pt2,oracleOutput)
-                price
-                payoffOutputLock
-            end
-          | _ -> autoFailw "Bad oracle output format"
+    let open ET in
+    do (pt0, dataOutput)   <-- tryAddPoint outpoint0 utxo;
+    do (pt1, tokenOutput)  <-- tryAddPoint outpoint1 utxo;
+    do (pt2, oracleOutput) <-- tryAddPoint outpoint2 utxo;
+    let dataToHash =
+      (Data4 nUnderlyingAssetBytes 1 1 1
+        (ByteArray nUnderlyingAssetBytes underlyingBytes)
+        (UInt64 price)
+        (UInt64 timestamp)
+        (Hash nonce)) in
+    // Validate data about the underlying against the Oracle's commitment
+    do expectedRoot <-- findRoot dataToHash auditPath;
+    match oracleOutput with
+    | { lock=(ContractLock oHash 1 (Hash mroot));
+        spend={asset=oHash2} } ->
+          do oracleHash <-- retT @ oracleHash;
+          if oHash <> oracleHash then autoFailw "Incorrect oracle ID" else
+          if oHash2 <> oracleHash then autoFailw "Wrong oracle asset type" else
+          if not (expectedRoot = mroot) then autoFailw "wrong root" else
+          if nUnderlyingAssetBytes <> 32
+          then autoFailw "Limitation: symbol must be 32 bytes." else begin
+          do underlyingSymbol <-- retT @ underlyingSymbol;
+          if underlyingBytes <> underlyingSymbol
+          then autoFailw "Trying to use the wrong underlying!" else
+          restOfEx cHash
+                   (pt0,dataOutput) (pt1,tokenOutput) (pt2,oracleOutput)
+                   price
+                   payoffOutputLock
           end
+    | _ -> autoFailw "Bad oracle output format"
 
 val cf': inputMsg -> nat -> cost nat 58
-let cf' iMsg k =
-  let open M in
+let cf' iMsg k = let open M in
   ret (k +
   begin match iMsg with
-  | { cmd = 0uy ; data = (| _ , Outpoint pt |) } -> 55
-  | { cmd = 1uy ; data = (| _ , OutpointVector 2 _ |) } -> 129
-  | { cmd = 2uy ; data = (| _ , Data2 _ _ (OutpointVector 2 _) (OutputLock lk) |) } -> 146
+  | { cmd = 0uy ; data = (| _ , Outpoint pt |) } -> 56
+  | { cmd = 1uy ; data = (| _ , OutpointVector 2 _ |) } -> 130
+  | { cmd = 2uy ; data = (| _ , Data2 _ _ (OutpointVector 2 _) (OutputLock lk) |) } -> 147
   | { cmd = 3uy ;
-    data =
-      (|
-        _ ,
-        Data4
-          _
-          _
-          _
-          _
-          _
-          (Data4 _ _ _ _ (ByteArray nUnderlyingAssetBytes _) _ _ _)
-          (Data2 _ _ _ (HashArray nAuditPathHashes _))
-          _
-      |) }
-    ->
-    (nUnderlyingAssetBytes + 3) * 384 + 1291 + nAuditPathHashes
+      data=(| _, Data4 _ _ _ _
+                   _
+                   (Data4 _ _ _ _ (ByteArray nUnderlyingAssetBytes _) _ _ _)
+                   (Data2 _ _ _ (HashArray nAuditPathHashes _))
+                   _ |) } ->
+                     (nUnderlyingAssetBytes + 3) * 384 + 1292 + nAuditPathHashes
   | _ -> 0
   end)
 
@@ -439,25 +379,16 @@ let cf i = cf' i 105
 val cf_lemma: i:inputMsg -> Lemma (let open M in
    force (cf i) == 105 +
    begin match i with
-   | { cmd = 0uy ; data = (| _ , Outpoint pt |) } -> 55
-   | { cmd = 1uy ; data = (| _ , OutpointVector 2 _ |) } -> 129
-   | { cmd = 2uy ; data = (| _ , Data2 _ _ (OutpointVector 2 _) (OutputLock lk) |) } -> 146
+   | { cmd = 0uy ; data = (| _ , Outpoint pt |) } -> 56
+   | { cmd = 1uy ; data = (| _ , OutpointVector 2 _ |) } -> 130
+   | { cmd = 2uy ; data = (| _ , Data2 _ _ (OutpointVector 2 _) (OutputLock lk) |) } -> 147
    | { cmd = 3uy ;
-     data =
-       (|
-         _ ,
-         Data4
-           _
-           _
-           _
-           _
-           _
-           (Data4 _ _ _ _ (ByteArray nUnderlyingAssetBytes _) _ _ _)
-           (Data2 _ _ _ (HashArray nAuditPathHashes _))
-           _
-       |) }
-     ->
-     (nUnderlyingAssetBytes + 3) * 384 + 1291 + nAuditPathHashes
+       data=(| _, Data4 _ _ _ _
+                    _
+                    (Data4 _ _ _ _ (ByteArray nUnderlyingAssetBytes _) _ _ _)
+                    (Data2 _ _ _ (HashArray nAuditPathHashes _))
+                    _ |) } ->
+                      (nUnderlyingAssetBytes + 3) * 384 + 1292 + nAuditPathHashes
    | _ -> 0
    end)
 let cf_lemma = function
@@ -465,53 +396,33 @@ let cf_lemma = function
   | { cmd = 1uy ; data = (| _ , OutpointVector 2 _ |) } -> ()
   | { cmd = 2uy ; data = (| _ , Data2 _ _ (OutpointVector 2 _) (OutputLock lk) |) } -> ()
   | { cmd = 3uy ;
-    data =
-      (|
-        _ ,
-        Data4
-          _
-          _
-          _
-          _
-          _
-          (Data4 _ _ _ _ (ByteArray nUnderlyingAssetBytes _) _ _ _)
-          (Data2 _ _ _ (HashArray nAuditPathHashes _))
-          _
-      |) }
-    -> ()
+      data=(| _, Data4 _ _ _ _
+                   _
+                   (Data4 _ _ _ _ (ByteArray nUnderlyingAssetBytes _) _ _ _)
+                   (Data2 _ _ _ (HashArray nAuditPathHashes _))
+                   _ |) } -> ()
   | _ -> ()
 
-
 val main : i:inputMsg -> cost (result transactionSkeleton) (force (cf i))
-let main i =
+let main i = let open M in
   cf_lemma i;
   do command <-- makeCommand i ;
   match command with
   | Initialize pointed ->
       initializeTx i.utxo i.contractHash pointed
-      <: (cost (result transactionSkeleton)
-         (let open M in
-          match i with
-          | { cmd = 0uy ; data = (| _ , Outpoint pt |) } -> 55
-          | { cmd = 1uy ; data = (| _ , OutpointVector 2 _ |) } -> 129
-          | { cmd = 2uy ; data = (| _ , Data2 _ _ (OutpointVector 2 _) (OutputLock lk) |) } -> 146
+      <: cost (result transactionSkeleton)
+         (match i with
+          | { cmd = 0uy ; data = (| _ , Outpoint pt |) } -> 56
+          | { cmd = 1uy ; data = (| _ , OutpointVector 2 _ |) } -> 130
+          | { cmd = 2uy ; data = (| _ , Data2 _ _ (OutpointVector 2 _) (OutputLock lk) |) } -> 147
           | { cmd = 3uy ;
-            data =
-              (|
-                _ ,
-                Data4
-                  _
-                  _
-                  _
-                  _
-                  _
-                  (Data4 _ _ _ _ (ByteArray nUnderlyingAssetBytes _) _ _ _)
-                  (Data2 _ _ _ (HashArray nAuditPathHashes _))
-                  _
-              |) }
-            ->
-            (nUnderlyingAssetBytes + 3) * 384 + 1291 + nAuditPathHashes
-          | _ -> 0))
+              data=(| _, Data4 _ _ _ _
+                           _
+                           (Data4 _ _ _ _ (ByteArray nUnderlyingAssetBytes _) _ _ _)
+                           (Data2 _ _ _ (HashArray nAuditPathHashes _))
+                           _ |) } ->
+                             (nUnderlyingAssetBytes + 3) * 384 + 1292 + nAuditPathHashes
+          | _ -> 0)
   | Collateralize V[pointed ; pointed'] ->
       collateralizeTx i.utxo i.contractHash pointed pointed'
   | Buy V[ptd ; ptd'] lk ->
